$\mathbf{e}_{0}$
$$
\begin{align}
&+  a^{0} \left(-\left(b^{01}\right)^{2} - \left(b^{02}\right)^{2} - \left(b^{03}\right)^{2} + \left(b^{12}\right)^{2} + \left(b^{13}\right)^{2} + \left(b^{23}\right)^{2} - p^{2} +  s^{2} \right)\\
&+ 2a^{1} \left(b^{01} s - b^{02} b^{12} - b^{03} b^{13} + b^{23} p\right)\\
&+ 2a^{2} \left(b^{01} b^{12} + b^{02} s - b^{03} b^{23} - b^{13} p\right)\\
&+ 2a^{3} \left(b^{01} b^{13} + b^{02} b^{23} + b^{03} s + b^{12} p\right)
\end{align}
$$

$\mathbf{e}_{1}$
$$
\begin{align}
&+ 2a^{0} \left(- b^{01} s - b^{02} b^{12} - b^{03} b^{13} - b^{23} p\right)\\
&+  a^{1} \left(- \left(b^{01}\right)^{2} + \left(b^{02}\right)^{2} + \left(b^{03}\right)^{2} - \left(b^{12}\right)^{2} - \left(b^{13}\right)^{2} + \left(b^{23}\right)^{2} - p^{2} + s^{2}\right)\\
&+ 2a^{2} \left(- b^{01} b^{02} + b^{03} p + b^{12} s - b^{13} b^{23}\right)\\
&+ 2a^{3} \left(- b^{01} b^{03} - b^{02} p + b^{12} b^{23} + b^{13} s\right)\\
\end{align}
$$

$\mathbf{e}_{2}$
$$
\begin{align}
&+ 2a^{0} \left(b^{01} b^{12} - b^{02} s - b^{03} b^{23} + b^{13} p\right)\\
&+ 2a^{1} \left(- b^{01} b^{02} - b^{03} p - b^{12} s - b^{13} b^{23}\right)\\
&+  a^{2} \left(\left(b^{01}\right)^{2} - \left(b^{02}\right)^{2} + \left(b^{03}\right)^{2} - \left(b^{12}\right)^{2} + \left(b^{13}\right)^{2} - \left(b^{23}\right)^{2} - p^{2} + s^{2}\right)\\
&+ 2a^{3} \left(b^{01} p - b^{02} b^{03} - b^{12} b^{13} + b^{23} s \right)\\
\end{align}
$$

$\mathbf{e}_{3}$
$$
\begin{align}
&+ 2a^{0} \left( b^{01} b^{13} + b^{02} b^{23} - b^{03} s - b^{12} p\right)\\
&+ 2a^{1} \left(-b^{01} b^{03} + b^{02} p + b^{12} b^{23} - b^{13} s\right)\\
&+ 2a^{2} \left(-b^{01} p - b^{02} b^{03} - b^{12} b^{13} - b^{23} s\right)\\
&+  a^{3} \left(\left(b^{01}\right)^{2} + \left(b^{02}\right)^{2} - \left(b^{03}\right)^{2} + \left(b^{12}\right)^{2} - \left(b^{13}\right)^{2} - \left(b^{23}\right)^{2} - p^{2} + s^{2}\right)\\
\end{align}
$$

==============================

$$
s  - b^{01} \mathbf{e}_{0}\wedge \mathbf{e}_{1} - b^{02} \mathbf{e}_{0}\wedge \mathbf{e}_{2} - b^{03} \mathbf{e}_{0}\wedge \mathbf{e}_{3} - b^{12} \mathbf{e}_{1}\wedge \mathbf{e}_{2} - b^{13} \mathbf{e}_{1}\wedge \mathbf{e}_{3} 
- b^{23} \mathbf{e}_{2}\wedge \mathbf{e}_{3} + p^{0123} \mathbf{e}_{0}\wedge \mathbf{e}_{1}\wedge \mathbf{e}_{2}\wedge \mathbf{e}_{3}
$$

$$
\left ( a^{0} s + a^{1} b^{01} + a^{2} b^{02} + a^{3} b^{03}\right ) \mathbf{e}_{0} + \left ( - a^{0} b^{01} + a^{1} s + a^{2} b^{12} + a^{3} b^{13}\right ) \mathbf{e}_{1} + \left ( - a^{0} b^{02} - a^{1} b^{12} + a^{2} s + a^{3} b^{23}\right ) \mathbf{e}_{2} + \left ( - a^{0} b^{03} - a^{1} b^{13} - a^{2} b^{23} + a^{3} s\right ) \mathbf{e}_{3} + \left ( a^{0} b^{12} - a^{1} b^{02} + a^{2} b^{01} + a^{3} p^{0123}\right ) \mathbf{e}_{0}\wedge \mathbf{e}_{1}\wedge \mathbf{e}_{2} + \left ( a^{0} b^{13} - a^{1} b^{03} - a^{2} p^{0123} + a^{3} b^{01}\right ) \mathbf{e}_{0}\wedge \mathbf{e}_{1}\wedge \mathbf{e}_{3} + \left ( a^{0} b^{23} + a^{1} p^{0123} - a^{2} b^{03} + a^{3} b^{02}\right ) \mathbf{e}_{0}\wedge \mathbf{e}_{2}\wedge \mathbf{e}_{3} + \left ( - a^{0} p^{0123} + a^{1} b^{23} - a^{2} b^{13} + a^{3} b^{12}\right ) \mathbf{e}_{1}\wedge \mathbf{e}_{2}\wedge \mathbf{e}_{3}
$$

$$\left ( \left(b^{01}\right)^{2} + \left(b^{02}\right)^{2} + \left(b^{03}\right)^{2} + \left(b^{12}\right)^{2} + \left(b^{13}\right)^{2} + \left(b^{23}\right)^{2} + \left(p^{0123}\right)^{2} + s^{2}\right )  + \left ( - 2 b^{01} 
b^{23} + 2 b^{02} b^{13} - 2 b^{03} b^{12} + 2 p^{0123} s\right ) \mathbf{e}_{0}\wedge \mathbf{e}_{1}\wedge \mathbf{e}_{2}\wedge \mathbf{e}_{3}
$$
